checkpoint end-to-end theorems with recovery for simple parts of FS.v

src/FS.v
@@ -6,6 +6,12 @@ Require Import BasicProg.
 Require Import Bool.
 Require Import Pred.
 Require Import Dir.
+Require Import Hoare.
+Require Import GenSep.
+Require Import SepAuto.
+Require Import Idempotent.
+
+Set Implicit Arguments.
 
 Definition file_len T lxp ixp inum rx : prog T :=
   ms <- MEMLOG.begin lxp;
@@ -18,6 +24,147 @@ Definition read_block T lxp ixp inum off rx : prog T :=
   b <- BFILE.bfread lxp ixp inum off ms;
   _ <- MEMLOG.commit lxp ms;
   rx b.
+
+Theorem read_block_ok : forall lxp bxp ixp inum off,
+  {< m F flist A f B v,
+  PRE    MEMLOG.rep lxp (NoTransaction m) ms_empty *
+         [[ (F * BFILE.rep bxp ixp flist)%pred (list2mem m) ]] *
+         [[ (A * inum |-> f)%pred (list2mem flist) ]] *
+         [[ (B * off |-> v)%pred (list2mem (BFILE.BFData f)) ]]
+  POST:r MEMLOG.rep lxp (NoTransaction m) ms_empty *
+         [[ r = v ]]
+  CRASH  MEMLOG.log_intact lxp m
+  >} read_block lxp ixp inum off.
+Proof.
+(* XXX why doesn't this proof, which unfolds MEM.log_intact first, go through?
+  unfold read_block, MEMLOG.log_intact.
+  hoare.
+  admit.
+  unfold MEMLOG.log_intact; cancel.
+*)
+
+  unfold read_block.
+  hoare.
+  admit.
+  unfold MEMLOG.log_intact; cancel.
+  unfold MEMLOG.log_intact; cancel.
+Qed.
+
+Theorem read_block_recover_ok : forall lxp bxp ixp inum off,
+  {< m F flist A f B v,
+  PRE     MEMLOG.rep lxp (NoTransaction m) ms_empty *
+          [[ (F * BFILE.rep bxp ixp flist)%pred (list2mem m) ]] *
+          [[ (A * inum |-> f)%pred (list2mem flist) ]] *
+          [[ (B * off |-> v)%pred (list2mem (BFILE.BFData f)) ]]
+  POST:r  MEMLOG.rep lxp (NoTransaction m) ms_empty *
+          [[ r = v ]]
+  CRASH:_ MEMLOG.rep lxp (NoTransaction m) ms_empty
+  >} read_block lxp ixp inum off >> MEMLOG.recover lxp.
+Proof.
+  intros.
+  unfold forall_helper; intros m F flist A f B v.
+  exists (MEMLOG.log_intact lxp m).
+
+  intros.
+  eapply pimpl_ok3.
+  eapply corr3_from_corr2.
+  eapply read_block_ok.
+  eapply MEMLOG.recover_ok.
+
+  cancel.
+  step.
+  cancel.
+  cancel.
+  rewrite crash_xform_sep_star_dist.
+  instantiate (a:=m). instantiate (a0:=m).
+  admit.
+
+  step.
+  admit.
+Qed.
+
+Definition write_block_inbounds T lxp ixp inum off v rx : prog T :=
+  ms <- MEMLOG.begin lxp;
+  ms <- BFILE.bfwrite lxp ixp inum off v ms;
+  ok <- MEMLOG.commit lxp ms;
+  rx ok.
+
+Theorem write_block_inbounds_ok : forall lxp bxp ixp inum off v,
+  {< m F flist A f B v0,
+  PRE     MEMLOG.rep lxp (NoTransaction m) ms_empty *
+          [[ (F * BFILE.rep bxp ixp flist)%pred (list2mem m) ]] *
+          [[ (A * inum |-> f)%pred (list2mem flist) ]] *
+          [[ (B * off |-> v0)%pred (list2mem (BFILE.BFData f)) ]]
+  POST:ok [[ ok = false ]] * MEMLOG.rep lxp (NoTransaction m) ms_empty \/
+          [[ ok = true ]] * exists m' flist' f',
+          MEMLOG.rep lxp (NoTransaction m') ms_empty *
+          [[ (F * BFILE.rep bxp ixp flist')%pred (list2mem m') ]] *
+          [[ (A * inum |-> f')%pred (list2mem flist') ]] *
+          [[ (B * off |-> v)%pred (list2mem (BFILE.BFData f')) ]]
+  CRASH   MEMLOG.log_intact lxp m \/ exists m' flist' f',
+          MEMLOG.log_intact lxp m' *
+          [[ (F * BFILE.rep bxp ixp flist')%pred (list2mem m') ]] *
+          [[ (A * inum |-> f')%pred (list2mem flist') ]] *
+          [[ (B * off |-> v)%pred (list2mem (BFILE.BFData f')) ]]
+  >} write_block_inbounds lxp ixp inum off v.
+Proof.
+  unfold write_block_inbounds.
+  hoare.
+  admit.
+  unfold MEMLOG.log_intact; cancel.
+  unfold MEMLOG.log_intact; cancel.
+Qed.
+
+Theorem write_block_inbounds_recover_ok : forall lxp bxp ixp inum off v,
+  {< m F flist A f B v0,
+  PRE     MEMLOG.rep lxp (NoTransaction m) ms_empty *
+          [[ (F * BFILE.rep bxp ixp flist)%pred (list2mem m) ]] *
+          [[ (A * inum |-> f)%pred (list2mem flist) ]] *
+          [[ (B * off |-> v0)%pred (list2mem (BFILE.BFData f)) ]]
+  POST:ok [[ ok = false ]] * MEMLOG.rep lxp (NoTransaction m) ms_empty \/
+          [[ ok = true ]] * exists m' flist' f',
+          MEMLOG.rep lxp (NoTransaction m') ms_empty *
+          [[ (F * BFILE.rep bxp ixp flist')%pred (list2mem m') ]] *
+          [[ (A * inum |-> f')%pred (list2mem flist') ]] *
+          [[ (B * off |-> v)%pred (list2mem (BFILE.BFData f')) ]]
+  CRASH:_ MEMLOG.rep lxp (NoTransaction m) ms_empty \/ exists m' flist' f',
+          MEMLOG.rep lxp (NoTransaction m') ms_empty *
+          [[ (F * BFILE.rep bxp ixp flist')%pred (list2mem m') ]] *
+          [[ (A * inum |-> f')%pred (list2mem flist') ]] *
+          [[ (B * off |-> v)%pred (list2mem (BFILE.BFData f')) ]]
+  >} write_block_inbounds lxp ixp inum off v >> MEMLOG.recover lxp.
+Proof.
+  intros.
+  unfold forall_helper; intros m F flist A f B v0.
+  exists (MEMLOG.log_intact lxp m \/ exists m' flist' f',
+          MEMLOG.log_intact lxp m' *
+          [[ (F * BFILE.rep bxp ixp flist')%pred (list2mem m') ]] *
+          [[ (A * inum |-> f')%pred (list2mem flist') ]] *
+          [[ (B * off |-> v)%pred (list2mem (BFILE.BFData f')) ]])%pred.
+
+  intros.
+  eapply pimpl_ok3.
+  eapply corr3_from_corr2.
+  eapply write_block_inbounds_ok.
+  eapply MEMLOG.recover_ok.
+
+  cancel.
+  step.
+  cancel.
+  cancel.
+
+  cancel.
+  cancel.
+  cancel.
+
+  rewrite crash_xform_sep_star_dist.
+  rewrite crash_xform_or_dist.
+  cancel.
+  admit.
+  step.
+
+  (* ... *)
+Admitted.
 
 Definition write_block T lxp bxp ixp inum off v rx : prog T :=
   ms <- MEMLOG.begin lxp;
